UTP/ITree_Designs.thy
@@ -44,7 +44,7 @@ lemma Stop_pre [dpre]: "itree_pre Stop = (True)\<^sub>e"
   by (auto simp add: itree_pre_def fun_eq_iff deadlock_def)
 
 lemma seq_pre [dpre]: "itree_pre (P ;; Q) = (itree_pre P \<and> wlp P (itree_pre Q))\<^sub>e"
-  apply (expr_simp, auto elim!: trace_to_bindE simp add: seq_itree_def kleisli_comp_def itree_pre_def wlp_itree_def itree_rel_defs retvals_def)
+  apply (expr_simp, auto elim!: trace_to_bindE simp add: kcomp_itree_def itree_pre_def wlp_itree_def itree_rel_defs retvals_def)
   apply (metis bind_diverge trace_to_bind_left)
   apply (meson trace_to_bind)
   apply (metis trace_of_Sils trace_to_Nil trace_to_trans)
