UTP/ITree_Hoare.thy
@@ -109,7 +109,7 @@ lemma hl_skip' [hoare_safe]:
   using assms by (auto simp add: hoare_alt_def Skip_def, expr_simp)
 
 lemma hl_seq: "\<lbrakk> \<^bold>{P\<^bold>} S\<^sub>1 \<^bold>{Q\<^bold>}; \<^bold>{Q\<^bold>} S\<^sub>2 \<^bold>{R\<^bold>} \<rbrakk> \<Longrightarrow> \<^bold>{P\<^bold>} S\<^sub>1 ;; S\<^sub>2 \<^bold>{R\<^bold>}"
-  by (auto simp add: hoare_ret_def seq_itree_def kleisli_comp_def)
+  by (auto simp add: hoare_ret_def kcomp_itree_def)
 
 lemma hoare_seq_inv [hoare_safe]: "\<lbrakk> \<^bold>{P\<^bold>} S\<^sub>1 \<^bold>{P\<^bold>}; \<^bold>{P\<^bold>} S\<^sub>2 \<^bold>{P\<^bold>} \<rbrakk> \<Longrightarrow> \<^bold>{P\<^bold>} S\<^sub>1 ;; S\<^sub>2 \<^bold>{P\<^bold>}"
   by (simp add: hl_seq)
@@ -141,7 +141,7 @@ lemma hl_fwd_assign_mwb [hoare_safe]:
   assumes "mwb_lens x" "\<And> x\<^sub>0. \<^bold>{\<^bold>D(x) \<and> $x = e\<lbrakk>\<guillemotleft>x\<^sub>0\<guillemotright>/x\<rbrakk> \<and> P\<lbrakk>\<guillemotleft>x\<^sub>0\<guillemotright>/x\<rbrakk>\<^bold>} S \<^bold>{Q\<^bold>}" "`P \<longrightarrow> \<^bold>D(x)`"
   shows "\<^bold>{P\<^bold>} x := e ;; S \<^bold>{Q\<^bold>}"
   using assms
-  by (auto simp add: seq_itree_def hoare_alt_def assigns_def kleisli_comp_def, expr_simp)
+  by (auto simp add: kcomp_itree_def hoare_alt_def assigns_def, expr_simp)
      (metis (no_types, opaque_lifting) mwb_lens.put_put mwb_lens.weak_get_put mwb_lens_weak weak_lens.put_closure weak_lens.put_get)
 
 lemma hl_fwd_assign:
@@ -172,7 +172,7 @@ lemma hl_guard [hoare_safe]:
   assumes "\<^bold>{P \<and> Q\<^bold>} C \<^bold>{R\<^bold>}"
   shows "\<^bold>{P\<^bold>} \<exclamdown>Q! ;; C \<^bold>{R\<^bold>}"
   using assms
-  by (auto simp add: hoare_alt_def test_def seq_itree_def kleisli_comp_def)
+  by (auto simp add: hoare_alt_def test_def kcomp_itree_def)
      (meson nonterminates_iff retvals_deadlock)
 
 lemma hl_match [hoare_safe]:
