UTP/ITree_Procedure.thy
@@ -50,13 +50,13 @@ abbreviation (input) proc_ret_empty :: "'s \<Rightarrow> ('e, unit \<times> 's) 
 "proc_ret_empty \<equiv> proc_ret (())\<^sub>e"
 
 lemma ret_rbind [simp]: "proc_ret e ;; rbind x = x := e"
-  by (simp add: proc_ret_def rbind_def seq_itree_def kleisli_comp_def assigns_def expr_defs)
+  by (simp add: proc_ret_def rbind_def kcomp_itree_def assigns_def expr_defs)
 
 lemma ret_rbind' [simp]: "(P ;; proc_ret e) ;; rbind x = P ;; x := e"
   by (simp add: kcomp_assoc)
 
 lemma ret_drop [simp]: "proc_ret e ;; rdrop = Skip"
-  by (simp add: proc_ret_def rdrop_def Skip_def seq_itree_def kleisli_comp_def)
+  by (simp add: proc_ret_def rdrop_def Skip_def kcomp_itree_def)
 
 lemma ret_drop' [simp]: "(P ;; proc_ret e) ;; rdrop = P"
   by (simp add: kcomp_assoc)
@@ -128,7 +128,7 @@ lemma hl_proc_seq:
   assumes "H{P} C\<^sub>1 {Q}" "H{Q} C\<^sub>2 {ret. @(R ret)}"
   shows "H{P} C\<^sub>1 ;; C\<^sub>2 {ret. @(R ret)}"
   using assms
-  by (auto elim!:trace_to_bindE bind_RetE' simp add: hoare_rel_triple_def ret_pred_def seq_itree_def kleisli_comp_def)
+  by (auto elim!:trace_to_bindE bind_RetE' simp add: hoare_rel_triple_def ret_pred_def kcomp_itree_def)
      (metis trace_to_Nil)+
 
 lemma hl_proc_cond [hoare_safe]:
@@ -150,30 +150,30 @@ lemma hl_proc_call [hoare_safe]:
   assumes "\<And> v. H{P \<and> \<guillemotleft>v\<guillemotright> = e} C(v) ;; rbind x {Q}"
   shows "H{P} x := <C(e)> {Q}"
   using assms
-  by (auto simp add: hoare_alt_def proc_call_def seq_itree_def kleisli_comp_def)
+  by (auto simp add: hoare_alt_def proc_call_def kcomp_itree_def)
 
 lemma thl_proc_call [hoare_safe]: 
   assumes "\<And> v. H[P \<and> \<guillemotleft>v\<guillemotright> = e] C(v) ;; rbind x [Q]"
   shows "H[P] x := <C(e)> [Q]"
   using assms
   apply (auto simp add: thoare_triple_def hl_proc_call wp)
-  apply (auto simp add: proc_call_def taut_def seq_itree_def kleisli_comp_def)
-  apply (metis (mono_tags, lifting) SEXP_def kleisli_comp_def pre_terminates seq_itree_def wp_seq)
+  apply (auto simp add: proc_call_def taut_def kcomp_itree_def)
+  apply (metis (mono_tags, lifting) SEXP_def kcomp_itree_def pre_terminates wp_seq)
   done
 
 lemma hl_proc_call_nret [hoare_safe]: 
   assumes "\<And> v. H{P \<and> \<guillemotleft>v\<guillemotright> = e} C(v) ;; rdrop {Q}"
   shows "H{P} call C(e) {Q}"
   using assms
-  by (auto simp add: hoare_alt_def proc_call_nret_def seq_itree_def kleisli_comp_def)
+  by (auto simp add: hoare_alt_def proc_call_nret_def kcomp_itree_def)
 
 lemma thl_proc_call_nret [hoare_safe]: 
   assumes "\<And> v. H[P \<and> \<guillemotleft>v\<guillemotright> = e] C(v) ;; rdrop [Q]"
   shows "H[P] call C(e) [Q]"
   using assms
   apply (auto simp add: thoare_triple_def hl_proc_call_nret wp)
-  apply (auto simp add: proc_call_nret_def taut_def seq_itree_def kleisli_comp_def)
-  apply (metis (mono_tags, lifting) SEXP_def kleisli_comp_def pre_terminates seq_itree_def wp_seq)
+  apply (auto simp add: proc_call_nret_def taut_def kcomp_itree_def)
+  apply (metis (mono_tags, lifting) SEXP_def kcomp_itree_def pre_terminates wp_seq)
   done
 
 lemma hl_output_return [hoare_safe]: 
