ROOT
@@ -1,7 +1,5 @@
-session "Interaction_Trees" = "Shallow_Expressions_Z" +
+session "Interaction_Trees" = "Z_Toolkit" +
   options [timeout = 600, document = pdf, document_output = "output"]
-  sessions
-    Abstract_Prog_Syntax
   theories
     ITrees
   document_files
@@ -15,7 +13,9 @@ session "ITree_Simulation" in "simulation" = "Interaction_Trees" +
 session "ITree_UTP" in "UTP" = "Interaction_Trees" +
   options [timeout = 600, document = false]
   sessions
+    Abstract_Prog_Syntax
     "Circus_Toolkit"
+    "Shallow_Expressions_Z"
   theories
     ITree_UTP
     ITree_Countable_Nondeterminism
